WIP, going to refactor SimSymb

compose/SimSymbKept.v
@@ -16,4 +16,250 @@ Require Import MapsC.
 
 Set Implicit Arguments.
 
+Require Import SimDef SimSymb.
+Require Import SimMem.
+Require Import SimMemInj.
+
+Record t': Type := mk {
+  kept: ident -> Prop;
+  coverage: ident -> Prop;
+  wf: kept <1= coverage;
+}
+.
+
+Arguments mk kept coverage : clear implicits.
+
+Inductive sim_sk (ss: t') (sk_src sk_tgt: Sk.t): Prop :=
+| closed_intro
+    (COVERAGE: (ss.(coverage) <1= sk_tgt.(privs)))
+    (PRIVS: sk_tgt.(privs) <1= sk_src.(privs))
+    (NOCOVER: forall
+        id
+        (PUBS: ~ ss.(coverage) id)
+      ,
+        <<SIM: sim_odef (sk_src.(prog_defmap) ! id) (sk_tgt.(prog_defmap) ! id)>>)
+    (KEPT: forall
+        id
+        (KEPT: ss.(kept) id)
+      ,
+        <<EQ: sk_src.(prog_defmap) ! id = sk_tgt.(prog_defmap) ! id>>)
+    (DROPPED: forall
+        id
+        (DROPPED: ~ ss.(kept) id)
+      ,
+        <<NONE: sk_tgt.(prog_defmap) ! id = None>>)
+    (PUB: sk_src.(prog_public) = sk_tgt.(prog_public))
+    (MAIN: sk_src.(prog_main) = sk_tgt.(prog_main))
+.
+
+Inductive sim_skenv (sm0: SimMem.t) (ss: t') (skenv_src skenv_tgt: SkEnv.t): Prop :=
+| sim_skenv_intro
+    (COVERAGE: ss.(coverage) <1= skenv_tgt.(skenv_privs))
+    (PRIVS: skenv_tgt.(skenv_privs) <1= skenv_src.(skenv_privs))
+    (SIMSYMB1: forall
+        id blk_src blk_tgt delta
+        (SIMVAL: SimMem.sim_val sm0 (Vptr blk_src Ptrofs.zero true) (Vptr blk_tgt delta true))
+        (BLKSRC: skenv_src.(Genv.find_symbol) id = Some blk_src)
+      ,
+        <<DELTA: delta = Ptrofs.zero>> /\ <<BLKTGT: skenv_tgt.(Genv.find_symbol) id = Some blk_tgt>>
+                                          (* /\ <<KEPT: ss.(kept) id>> *)
+    )
+    (SIMSYMB2: forall
+        id
+        (KEPT: ss.(kept) id)
+        blk_src
+        (BLKSRC: skenv_src.(Genv.find_symbol) id = Some blk_src)
+      ,
+        exists blk_tgt,
+          <<BLKTGT: skenv_tgt.(Genv.find_symbol) id = Some blk_tgt>> /\
+           <<SIM: SimMem.sim_val sm0 (Vptr blk_src Ptrofs.zero true) (Vptr blk_tgt Ptrofs.zero true)>>)
+    (SIMSYMB3: forall
+        id blk_tgt
+        (BLKTGT: skenv_tgt.(Genv.find_symbol) id = Some blk_tgt)
+      ,
+        exists blk_src,
+          <<BLKSRC: skenv_src.(Genv.find_symbol) id = Some blk_src>>
+           /\ <<SIM: SimMem.sim_val sm0 (Vptr blk_src Ptrofs.zero true) (Vptr blk_tgt Ptrofs.zero true)>>
+             (* /\ <<KEPT: ss.(kept) id>> *)
+    )
+.
+
+Global Program Definition link_ss (ss0 ss1: t'): option t' :=
+  Some (mk (ss0.(kept) \1/ ss1.(kept)) (ss0.(coverage) \1/ ss1.(coverage)) _)
+.
+Next Obligation.
+  u; ii; ss.
+  destruct ss0, ss1; ss.
+  des; eauto.
+Qed.
+
+Global Program Instance Linker_t: Linker t' := {|
+  link := link_ss;
+  linkorder (ss0 ss1: t') := ss0.(kept) <1= ss1.(kept) /\ ss0.(coverage) <1= ss1.(coverage);
+|}.
+Next Obligation.
+  ss. split; ss.
+  - split; u; ii; ss; left; ss.
+  - split; u; ii; ss; right; ss.
+Qed.
+
+Global Program Instance SimSymbKept: SimSymb.class SimMemInj := {
+  t := t';
+  coverage := coverage;
+  (* kept := bot2; *)
+  sim_sk := sim_sk;
+  sim_skenv := sim_skenv;
+}
+.
+Next Obligation.
+  admit "".
+Qed.
+Next Obligation.
+  inv SIMSK.
+  econs; eauto.
+  - i.
+    destruct ss; ss.
+    destruct (classic (kept0 id)).
+    + erewrite KEPT; eauto.
+    + erewrite DROPPED in *; ss.
+Qed.
+Next Obligation.
+  admit "".
+Qed.
+Next Obligation.
+  admit "".
+Qed.
+Next Obligation.
+  admit "".
+Qed.
+(* Next Obligation. *)
+(*   inv SIMSKENV. *)
+(*   econs; eauto. *)
+(*   - i; ss. *)
+(*     exploit SIMSYMB1; eauto. i; des. esplits; eauto. *)
+(* Qed. *)
+Next Obligation.
+  inv SIMSKENV.
+  inv LESRC. inv LETGT.
+  econs; eauto.
+  -
+  - i. destruct ss; ss.
+    inv SIMSK; ss.
+    destruct (classic (defs sk_src id)); cycle 1.
+    { erewrite NPROJ in *; ss. }
+    exploit PROJ; eauto. i; des. rewrite BLKSRC in *.
+    exploit SIMSYMB1; eauto. i; des.
+    esplits; eauto.
+    destruct (classic (kept0 id)).
+    + erewrite <- PROJ0; eauto.
+      { hnf in H. des. erewrite KEPT in *; ss. hnf. esplits; eauto. }
+    + erewrite <- PROJ0; eauto.
+      esplits; eauto.
+    +
+      exploit KEPT; eauto. i ;des.
+      destruct sk_tgt.(prog_defmap) ! id eqn:T; cycle 1.
+      { exfalso. destruct ss; ss.
+      }
+      exploit PROJ; eauto. i; des_safe.
+      exploit PROJ0; eauto. i; des_safe.
+      rewrite <- H1. eapply SIMSYMB1; eauto.
+      rewrite BLKSRC in *. ss.
+    + exploit NPROJ; eauto. i; des_safe. rewrite BLKSRC in *. ss.
+  - i.
+    destruct ss; ss.
+    exploit PROJ; eauto.
+    exploit SIMSYMB2; eauto.
+Qed.
+  inv SIMSKENV.
+  econs; eauto.
+  - i. eapply SIMSYMB1; eauto. ss. inv 
+Qed.
+Next Obligation.
+  admit "".
+Qed.
+
+  inv SIMSK.
+  econs; eauto.
+  esplits; eauto. ss.
+Qed.
+Next Obligation.
+  inv SIMSK.
+  econs; ss; eauto.
+  - admit "easy. pull out as lemma".
+  - ii; ss.
+    unfold match_program in *.
+    generalize (Genv.globalenvs_match SIM); intro SIMGE.
+    inv SIMGE.
+    admit "this should hold.".
+  - inv SIM. des. ss.
+  - inv SIM. des. ss.
+Qed.
+Next Obligation.
+  exists tt.
+  split.
+  - ss.
+  - econs; eauto. inv CLOSED0. inv CLOSED1.
+  admit "This should hold".
+  Print TransfLink.
+  (* exploit link_match_program; eauto. *)
+Qed.
+(* Next Obligation. *)
+(*   inv CLOSED. clear_tac. *)
+(*   assert(SIMID: forall id, (prog_defmap sk_src) ! id = (prog_defmap sk_tgt) ! id). *)
+(*   { i. eapply NOCOVER; eauto. } clear NOCOVER. *)
+(*   u. ss. *)
+(*   econs; eauto. *)
+(*   - admit "this should hold, if not, 1) add uniqueness condition on good_prog to make it hold. *)
+(* 2) Replace Genv.globalenv with my_globalenv, which makes it unique". *)
+(*   - intro id. *)
+(*     specialize (SIMID id). *)
+(*     generalize Genv.find_def_symbol. intro LEMMA. *)
+(*     destruct ((prog_defmap sk_src) ! id) eqn:T. *)
+(*     + eapply LEMMA in T. symmetry in SIMID. eapply LEMMA in SIMID. des. *)
+(*       rewrite T. rewrite SIMID. ss. *)
+(*     + *)
+(*     admit "this should hold, if not, add uniqueness condition on good_prog to make it hold.". *)
+(*     ss. *)
+(* Qed. *)
+
+
+
+
+Next Obligation.
+  eexists (SimMemId.mk _ _).
+  esplits; ss; eauto.
+  u. inv SIMSK.
+  Print Genv.init_mem_transf.
+  Print Genv.init_mem_transf_partial.
+  About Genv.init_mem_match.
+  exploit (Genv.init_mem_match SIM); eauto. i. clarify.
+  econs; eauto.
+  - admit "easy; Genv.init_mem_genv_next".
+  - i. admit "this should hold... Genv.find_symbol_match".
+Qed.
+(* Next Obligation. *)
+(*   inv CLOSED. *)
+(*   unfold match_program in *. *)
+(*   generalize (Genv.globalenvs_match SIM); intro SIMGE. *)
+(*   inv SIMGE. *)
+(*   econs; eauto. *)
+(* Qed. *)
+Next Obligation.
+  inv LESRC.
+  inv LETGT.
+  inv SIMSKENV.
+  econs; eauto.
+  - eq_closure_tac.
+  - intro id.
+    destruct (Classical_Prop.classic (pubs id)); cycle 1.
+    + exploit NPROJ; eauto. { ii; des; eauto. } i; des.
+      exploit NPROJ0; eauto. { ii; des; eauto. } i; des.
+      eq_closure_tac. (* TODO: debug this *)
+      rewrite H0. rewrite H1. ss.
+    + exploit PROJ; eauto. i; des.
+      exploit PROJ0; eauto. i; des.
+      eq_closure_tac. (* TODO: debug this *)
+      rewrite <- H0. rewrite <- H1.
+      ss.
+Qed.
 
